src/tls/TLSMem.fst
@@ -6,3 +6,19 @@ include FStar.ST
 include FStar.All
 
 let hh_as_ref = HyperHeap.as_ref
+
+(* TODO:
+ - regions from Parse
+ - colors: replace with stateful operator giving a fresh color
+*)
+
+assume val fresh_color: unit -> ST color (requires (fun h -> True)) (ensures (fun h c h1 -> c not in h /\ c in h1)) // TODO: implement
+
+private
+let tls_color_epoch_color_hs_color =
+  let t = fresh_color () in
+  let e = fresh_color () in
+  let h = fresh_color () in
+  (t, e, h)
+
+let tls_color = let (t, _, _) = tls_color_epoch_color_hs_color in t
